Prove lease_acc_update

src/program_proof/minlease/proof.v
@@ -4,27 +4,85 @@ From Perennial.program_proof Require Import proof_prelude.
 From Perennial.goose_lang.ffi Require Export grove_ffi_time_axiom.
 From Perennial.base_logic.lib Require Import ghost_var.
 From Goose.github_com.mit_pdos.gokv Require Import minlease.
+From iris.bi.lib Require Import fixpoint.
+From Perennial.base_logic Require Import lib.saved_prop.
 
 Section proof.
 
 Context `{!heapGS Σ}.
 Context `{!ghost_varG Σ u64}.
+Context `{!savedPropG Σ }.
 
 Context {γtime:gname}.
+
 Notation is_time_lb := (is_time_lb γtime).
 Notation own_time := (own_time γtime).
 
 (* Q is the lease obligation *)
 Definition underLease (N:namespace) (leaseExpiration:u64) (P:iProp Σ) (Q:iProp Σ) : iProp Σ :=
-  ∀ (t:u64),
-  ⌜int.nat t < int.nat leaseExpiration⌝ →
-  own_time t ={↑N}=∗
-  (P ∗ (P ={↑N}=∗ own_time t))
-.
-(* inv N (P ∨ is_time_lb leaseExpiration) *)
+  ∃ γprop,
+  saved_prop_own γprop (DfracOwn (1/2)) P ∗
+  inv N (∃ P',
+    saved_prop_own γprop (DfracOwn (1/2)) P' ∗
+    (P' ∗ (P' -∗ Q) ∨ is_time_lb leaseExpiration)
+  ).
 
-Definition postLease (N:namespace) (leaseExpiration:u64) (P:iProp Σ) :=
-  is_time_lb leaseExpiration ={↑N}=∗ P
+Lemma underLease_mono P' P Q e N :
+  (P -∗ P') -∗
+  (P' -∗ Q) -∗
+  underLease N e P Q -∗
+  underLease N e P' Q
+.
+Proof.
+Admitted.
+
+Lemma lease_acc_update N e P Q :
+  underLease N e P Q -∗
+  £ 1 -∗
+  £ 1 -∗
+  ∀ (t:u64),
+  ⌜int.nat t < int.nat e⌝ →
+  own_time t ={↑N,∅}=∗
+  (P ∗ (∀ P', P' -∗ (P' -∗ Q) ={∅,↑N}=∗ own_time t ∗ underLease N e P' Q))
+.
+Proof.
+  iIntros "Hlease Hlc Hlc2".
+  iIntros (?) "%Hineq Htime".
+  iDestruct "Hlease" as (γprop) "[Hprop #Hinv]".
+  iInv "Hinv" as "Hi" "Hclose".
+  iMod (lc_fupd_elim_later with "Hlc Hi") as "Hi".
+  iDestruct "Hi" as (?) "[Hprop2 Hi]".
+  iDestruct (saved_prop_agree with "Hprop Hprop2") as "#Hagree1".
+  iMod (lc_fupd_elim_later with "Hlc2 Hagree1") as "#Hagree".
+  replace (↑N ∖ ↑N) with (∅:coPset) by set_solver.
+  iModIntro.
+  iDestruct "Hi" as "[[HP HQwand]| Hbad]"; last first.
+  {
+    iDestruct (mono_nat_lb_own_valid with "Htime Hbad") as %[_ Hbad].
+    exfalso.
+    word.
+  }
+  iSplitL "HP".
+  {
+    by iRewrite "Hagree".
+  }
+  iIntros (R) "HR HRwandQ".
+  iMod (saved_prop_update_2 R with "Hprop Hprop2") as "[Hprop Hprop2]".
+  { apply Qp.half_half. }
+  iFrame "Htime".
+  iMod ("Hclose" with "[HRwandQ HR Hprop2]").
+  {
+    iNext.
+    iExists _; iFrame "Hprop2".
+    iLeft.
+    iFrame.
+  }
+  iModIntro.
+  iExists _; iFrame "∗#".
+Qed.
+
+Definition postLease (N:namespace) (leaseExpiration:u64) (Q:iProp Σ) :=
+  is_time_lb leaseExpiration ={↑N}=∗ Q
 .
 
 (* P are resources you can access and modify at the moment you check that the
